Implement Parse_helloRetryRequest

targets/tls13/Parse_helloRetryRequest.fsti
@@ -12,7 +12,22 @@ module U32 = FStar.UInt32
 module LP = LowParse.SLow.Base
 module L = FStar.List.Tot
 
-type helloRetryRequest_extensions = l:list extension{0 <= L.length l /\ L.length l <= 16383}
+type helloRetryRequest_extensions_raw = l:list extension
+
+val helloRetryRequest_extensions_byteSize: helloRetryRequest_extensions_raw -> GTot nat
+
+inline_for_extraction
+val helloRetryRequest_extensions_byteSize32: (x: helloRetryRequest_extensions_raw) -> Tot (y: U32.t {
+  let sz = helloRetryRequest_extensions_byteSize x in
+  if sz > U32.v (LP.u32_max)
+  then y == LP.u32_max
+  else U32.v y == sz
+} )
+
+type helloRetryRequest_extensions = (l: helloRetryRequest_extensions_raw { 
+  let sz = helloRetryRequest_extensions_byteSize l in
+  0 <= sz /\ sz <= 65535
+})
 
 type helloRetryRequest = {
 	server_version : protocolVersion;
@@ -20,8 +35,6 @@ type helloRetryRequest = {
 	selected_group : namedGroup;
 	extensions : helloRetryRequest_extensions;
 }
-
-val bytesize: helloRetryRequest -> nat
 
 inline_for_extraction val helloRetryRequest_parser_kind_metadata : LP.parser_kind_metadata_t
 
@@ -35,3 +48,4 @@ val helloRetryRequest_serializer: LP.serializer helloRetryRequest_parser
 
 inline_for_extraction val helloRetryRequest_serializer32: LP.serializer32 helloRetryRequest_serializer
 
+val helloRetryRequest_size32: LP.size32 helloRetryRequest_serializer
