targets/tls13/Parse_protocolVersion.fst
@@ -9,4 +9,3 @@ module LP = LowParse.SLow
 module L = FStar.List.Tot
 
 #reset-options "--using_facts_from '* -FStar.Tactics -FStar.Reflection' --z3rlimit 16 --z3cliopt smt.arith.nl=false --max_fuel 2 --max_ifuel 2"
-
